Analysis/definitions.dfy
@@ -1,0 +1,319 @@
+
+module Analysis {
+    /**type defs */
+    type pos = x: nat | 1 <= x witness 1
+
+    /** axioms */
+    lemma CompletenessAxiomUpper(A: iset<real>, a: real)
+        requires exists p: real :: p in A 
+        requires upperBound(A, a)
+        // ensures exists k: real :: leastUpperBound(A, k) && upperBound(A, k)
+        ensures exists k: real :: sup(A, k)
+
+    lemma CompletenessAxiomLower(A: iset<real>, a: real)
+        requires exists p: real :: p in A 
+        requires lowerBound(A, a)
+        // ensures exists k: real :: greatestLeastBound(A, k) && lowerBound(A, k)
+        ensures exists k: real :: inf(A, k)
+
+    lemma MonotoneConvergenceThmInc(a_i: pos -> real)
+        requires MonotonicIncreasingSequence(a_i)
+        ensures (forall a: real :: !Limit(a_i, a)) || exists a: real :: sup(iset n: pos | true :: a_i(n), a) && Limit(a_i, a)
+
+
+    lemma MonotoneConvergenceThmDec(a_i: pos -> real)
+        requires MonotonicDecreasingSequence(a_i)
+        ensures (forall a: real :: !Limit(a_i, a)) || exists a: real :: inf(iset n: pos | true :: a_i(n), a) && Limit(a_i, a)
+
+    lemma WellOrderingPrinciple(s: iset<pos>)
+        requires s != iset{}
+        ensures exists min :: min in s && forall x | x in s && x != min :: min < x; 
+
+    /** functions */
+    function Range<T, U>(f: T -> U, A: set<T>): set<U> {
+        set x | x in A :: f(x)
+    }
+
+    function sub(a: real, b: real): real {
+        a - b
+    }
+
+    function add(a: real, b: real): real {
+        a+b
+    }
+
+    function prod(a: real, b: real): real {
+        a * b
+    }
+
+    function div(a: real, b: real): real 
+        requires b != 0.0
+    {
+        a / b
+    }
+
+    function abs(a: real): real {
+        if a >= 0.0 then a else -a
+    }
+
+    function SubSequenceOf(a_i: pos -> real, k_i: pos -> pos): pos -> real
+        requires MonotonicIncreasingPos(k_i)
+    {
+        (n: pos) => a_i(k_i(n))
+    }
+
+    function addSequence(a_i: pos -> real, b_i: pos -> real): pos -> real {
+        (n:pos) => a_i(n) + b_i(n)
+    }
+
+    function prodSequence(a_i: pos -> real, b_i: pos -> real): pos -> real {
+        (n:pos) => prod(a_i(n) , b_i(n))
+    }
+
+    function subSequence(a_i: pos -> real, b_i: pos -> real): pos -> real {
+        (n:pos) => a_i(n) - b_i(n)
+    }
+
+    function mulSequence(a_i: pos -> real, c: real): pos -> real {
+        (n:pos) => prod(c, a_i(n))
+    }
+
+    function maxNat(a: nat, b: nat): nat {
+        if a >= b then a else b
+    }
+
+    function maxReal(a: real, b: real): real {
+        if a >= b then a else b
+    }
+    /** predicates */
+    ghost predicate Injective<A(!new), B>(f: A -> B)
+    {
+        forall x, y :: x != y ==> f(x) != f(y)
+    }
+
+    ghost predicate isTotal<G(!new), B(!new)>(f:G -> B)
+        reads f.reads
+    {
+        forall g:G :: f.requires(g)
+    }
+
+    ghost predicate Surjective<A(!new), B(!new)>(f: A -> B) 
+        reads f.reads
+        // requires isTotal(f)
+    {
+        forall b: B :: exists a: A :: f(a) == b 
+    }
+
+    ghost predicate Bijective<A(!new), B(!new)>(f: A -> B) 
+    {
+        Injective(f) && Surjective(f)
+    }
+
+    ghost predicate upperBound(A: iset<real>, a: real) {
+        forall x :: x in A ==> x <= a    
+    }
+
+    ghost predicate lowerBound(A: iset<real>, b: real) {
+        forall x :: x in A ==> x >= b
+    }
+
+    ghost predicate leastUpperBound(A: iset<real>, a: real) 
+    {
+        forall epsilon: real :: epsilon > 0.0 ==> !upperBound(A, sub(a, epsilon))  
+    }
+
+    ghost predicate greatestLeastBound(A: iset<real>, b: real) {
+        forall epsilon: real :: epsilon > 0.0 ==> !lowerBound(A, add(b , epsilon))  
+    }
+
+    ghost predicate sup(A: iset<real>, a: real) {
+        upperBound(A, a) && leastUpperBound(A, a)
+    }
+
+    ghost predicate inf(A: iset<real>, b: real) {
+        lowerBound(A, b) && greatestLeastBound(A, b)
+    }
+
+    ghost predicate minimalElement(A: iset<real>, a: real) {
+        a in A && lowerBound(A, a)
+    }
+
+    ghost predicate maximalElement(A: iset<real>, a: real) {
+        a in A && upperBound(A, a)
+    }
+
+    predicate lessThanEqual(n: nat, x: real) {
+        n as real <= x
+    }
+    
+    predicate greaterThan(n: nat, x: real) {
+        n as real > x
+    }
+
+    predicate lessThan(n: nat, x: real) {
+        n as real < x
+    }
+
+    predicate positiveNat(x: nat) {
+        x > 0
+    }
+
+    predicate positiveReal(x: real) {
+        x > 0.0
+    }
+
+    predicate converges(a_i: pos -> real, n: pos, epsilon: real, a: real) {
+        abs(a_i(n)-a) < epsilon
+    }
+
+    predicate CauchyCriterion(a_i: pos -> real, epsilon: real, m: pos, n: pos) {
+        abs(a_i(m)-a_i(n)) < epsilon
+    }
+
+    ghost predicate isCauchy(a_i: pos -> real) {
+        forall epsilon: real :: positiveReal(epsilon) ==> exists N: nat :: positiveNat(N) && forall n: pos,m:pos :: m > n > N ==> CauchyCriterion(a_i, epsilon, m, n)
+    }
+
+    ghost predicate MonotonicIncreasingPos(k_i: pos -> pos) {
+        forall n,m :: n < m ==> k_i(n) < k_i(m)
+    }
+
+    ghost predicate MonotonicIncreasingSequence(a_i: pos -> real) {
+        forall n,m :: n < m ==> a_i(n) <= a_i(m)
+    }
+
+    ghost predicate MonotonicDecreasingSequence(a_i: pos -> real) {
+        forall n,m :: n < m ==> a_i(n) >= a_i(m)
+    }
+
+    ghost predicate Monotone(a_i: pos -> real) {
+        MonotonicIncreasingSequence(a_i) || MonotonicDecreasingSequence(a_i)
+    }
+    ghost predicate Limit(a_i: pos -> real, a: real) {
+        forall epsilon: real :: positiveReal(epsilon) ==> exists N: nat :: positiveNat(N) && forall n: pos :: n > N ==> converges(a_i, n, epsilon, a)
+    }
+
+    ghost predicate bounded(ss: iset<real>, L: real, U: real) {
+        forall x :: x in ss ==> L <= x <= U
+    }
+
+    ghost predicate boundedSeq(a_i: pos -> real, L: real, U: real) {
+        forall n:pos :: positiveNat(n) ==> L <= a_i(n) <= U
+    }
+
+    /** lemmas */
+    lemma ArchProof(x: real, a: real, b: real)
+        requires a > 0.0
+        requires x == b/a
+        ensures exists n: pos :: n as real > x
+    {
+        if x < 0.0 {
+            assert 1 as real > x;
+        }else{
+            assert b >= 0.0;
+            if forall n: pos :: n as real <= x {
+                var naturals: iset<real> := iset ns: nat | lessThanEqual(ns, x) :: ns as real;
+                // assert upperBound(naturals, x);
+                if x <= 1.0 {
+                    assert 2 as real > x;
+                    assert false;
+                }else{
+                    assert lessThanEqual(1, x);
+                    assert 1.0 in naturals;
+                }
+                CompletenessAxiomUpper(naturals, x);
+                var alpha: real :| leastUpperBound(naturals, alpha as real) && upperBound(naturals, alpha as real); 
+                var mp: nat := add(alpha , 1.0).Floor;
+                assert lessThanEqual(mp, x);
+                assert mp as real in naturals;
+                assert upperBound(naturals, mp as real);
+
+                assert false;
+            }
+        }
+    }
+
+    lemma ArchimedeanPrinciple(epsilon: real)
+        requires epsilon > 0.0
+        ensures exists n: pos :: 1.0 / (n as real) < epsilon
+    {
+        ArchProof(1.0 / epsilon, epsilon, 1.0);
+        var n: pos :| n as real > 1.0 / epsilon;
+        if epsilon >= 1.0 {
+        }else{
+            calc ==> {
+                n as real > 1.0 / epsilon;
+                {assert (n as real) *  epsilon > (1.0/epsilon)*epsilon;}
+                (n as real) * epsilon > 1.0;
+                epsilon > 1.0 / (n as real);
+            }
+        }
+    }
+
+    lemma TriangeInequality(a: real, b: real)
+        ensures abs(a+b) <= abs(a) + abs(b)
+    {
+    }
+
+    lemma SubSequenceOfMonotoneSequenceIsMonotone(a_i: pos -> real, k_i: pos -> pos, a: real)
+        requires MonotonicIncreasingPos(k_i)
+        requires Monotone(a_i)
+        ensures Monotone(SubSequenceOf(a_i, k_i))
+    {
+
+    }
+
+    lemma inequalitProduct(a: real, b: real, c: real)
+        requires a < b
+        requires c > 0.0
+        ensures c*a < c*b
+    {
+
+    }
+
+
+    lemma boundedEqual(a_i: pos -> real, a_range: iset<real>, L: real, U: real)
+        requires a_range == iset n: pos | positiveNat(n) :: a_i(n)
+        requires bounded(a_range, L, U)
+        ensures boundedSeq(a_i, L, U)
+    {
+        forall n:pos | positiveNat(n)
+            ensures L <= a_i(n) <= U
+        {
+            assert a_i(n) in a_range;
+        }
+
+    }
+
+    lemma boundedEqualLeft(a_i: pos -> real, a_range: iset<real>, L: real, U: real)
+        requires a_range == iset n: pos | positiveNat(n) :: a_i(n)
+        requires boundedSeq(a_i, L, U)
+        ensures bounded(a_range, L, U)
+    {}
+
+    lemma absProd(a: real, b: real)
+        ensures abs(prod(a,b)) == prod(abs(a), abs(b))
+    {}
+
+    lemma prodLessThan(a: real, b: real, c: real)
+        requires a > 0.0
+        requires 0.0 <= b < c 
+        ensures prod(a , b) < prod(a , c)
+    {}
+
+    lemma divSmaller(a: real, b: real)
+        requires a >= 0.0
+        requires b > a
+        ensures div(a,b) < 1.0
+    {
+        var diff := b-a;
+        assert a/(a+diff) < 1.0;
+    }
+
+    lemma divCommute(a: real, b: real, c: real)
+        requires c != 0.0
+        // ensures a * (b/c) == (a/c)*b
+        ensures prod(a , div(b,c)) == prod(div(a,c),b)
+    {
+    }
+}
