Analysis/exercises/cummings-ch1.dfy
@@ -1,0 +1,137 @@
+include "../definitions.dfy"
+module CummingsCh1 {
+    import opened Analysis
+
+lemma exercise1_5<T>(A: set<T>, B: set<T>)
+    requires A + B == A
+    ensures B <= A
+{
+
+}
+
+
+lemma exercise1_6<T,U>(f: T  -> U, f_inv: U -> T, B: set<U>)
+    requires forall u: U :: f(f_inv(u)) == u
+    ensures Range(f, Range(f_inv, B)) <= B
+{
+
+}
+
+lemma exercise1_6c<T,U>(f: T  -> U, f_inv: U -> T, A: set<T>)
+    // requires forall u: U :: f(f_inv(u)) == u
+    requires forall a: T :: a in A ==> f_inv(f(a)) == a
+    ensures A <= Range(f_inv, Range(f, A))
+{
+
+}
+
+lemma exercise1_7<X(!new), Y(!new)>(f: X -> Y, g: Y -> X)
+    requires forall x: X :: g(f(x)) == x
+    ensures Injective(f) && Surjective(g)
+{
+    if !Injective(f) {
+        var x,y: X :| x != y && f(x) == f(y);
+        assert g(f(x)) == g(f(y));
+        assert false;
+    } else if !Surjective(g) {
+        // assert exists b: Y :: !(exists a: X :: f(a) == b);
+        // assert !(forall b: X :: exists a: Y :: g(a) == b);
+        // var b: X :| !(exists a: Y :: g(a) == b);
+        var b: X :| forall a: Y :: g(a) != b;
+        assert g(f(b)) != b;
+        assert false;
+    }
+}
+
+lemma exercise1_23(A: iset<real>, B: iset<real>, abound: real, bbound: real, epsilon: real)
+    requires A <= B
+    requires sup(A, abound)
+    requires sup(B, bbound)
+    requires epsilon > 0.0
+    ensures abound <= bbound
+{
+  if abound > bbound {
+    var myepsilon := abound - bbound;
+    assert bbound == sub(abound, myepsilon);
+    assert upperBound(A, bbound);
+    assert upperBound(A, sub(abound, myepsilon));
+    assert  false;
+  }
+}
+
+lemma example1_25(A: iset<real>)
+    requires A == iset x: real | x < 0.0
+    ensures sup(A, 0.0)
+{
+    assert forall x: real :: x in A ==> x < 0.0;
+    assert upperBound(A, 0.0);
+    forall epsilon: real | epsilon > 0.0
+        ensures !upperBound(A, sub(0.0,epsilon))
+    {
+        calc ==> {
+            epsilon > 0.0;
+            - epsilon > -2.0 * epsilon;
+            (- epsilon)/2.0 > -epsilon;
+        }
+        assert (-epsilon)/2.0 in A;
+        assert (-epsilon)/2.0 > sub(0.0,epsilon);
+        // assert !upperBound(A, )
+    }
+    assert leastUpperBound(A, 0.0);
+}
+
+function e29(n: nat): real {
+    (n as real)/(n as real + 1.0)
+}
+
+lemma exercise1_29a(A: iset<real>)
+    requires A == iset n: pos :: e29(n)
+    ensures sup(A, 1.0)
+{
+    assert upperBound(A, 1.0);
+    forall epsilon: real | epsilon > 0.0 
+        ensures !upperBound(A, sub(1.0, epsilon))
+    {
+        ArchimedeanPrinciple(epsilon);
+        var n: pos :| 1.0 / (n as real) < epsilon; 
+        assert (1.0 / (n as real + 1.0)) < 1.0 / (n as real);
+        assert e29(n) in A;
+        assert sub(1.0, 1.0 / (n as real + 1.0)) == e29(n); 
+        // assert exists k :: k in A && k > sub(1.0, epsilon);
+    }
+}
+
+lemma exercise1_29b(A: iset<real>)
+    requires A == iset n: pos :: e29(n)
+    ensures inf(A, 1.0/2.0)
+{
+    assert e29(1) in A;
+    forall x | x in A 
+        ensures x >= 1.0/2.0
+    {
+        var n: nat :| x == e29(n);
+        if n == 1 {
+            assert x == 1.0/2.0;
+        }else{
+            assert (n as real)/(n as real + 1.0) >= 1.0/2.0;
+        }
+    }
+    assert lowerBound(A, 1.0/2.0);
+    assert greatestLeastBound(A, 1.0/2.0);
+}
+
+lemma exercise1_30(A: iset<real>, B: iset<real>, abound: real, bbound: real)
+    requires sup(A, abound)
+    requires sup(B, bbound)
+    requires abound < bbound
+    ensures exists b: real :: b in B && upperBound(A, b)
+{
+    // assert upperBound(A, bbound);
+    // assert leastUpperBound(B, bbound);
+    // assert forall epsilon: real :: epsilon > 0.0 ==> !upperBound(B, sub(bbound, epsilon));
+    var epsilon := sub(bbound, abound);
+    // assert abound + epsilon == bbound;
+    // assert epsilon > 0.0;
+    assert !upperBound(B, sub(bbound, epsilon));
+}
+}
