Analysis/exercises/cummings-ch3.dfy
@@ -1,0 +1,363 @@
+include "../definitions.dfy"
+module CummingsCh3 {
+    import opened Analysis
+
+    lemma exercise3_1b(a_i: pos -> real, N: nat)
+        requires Limit(a_i, 0.001)
+        requires positiveNat(N) && forall n :: n > N ==> converges(a_i, n, 0.001, 0.001)
+        ensures forall n:: n > N ==> a_i(n) >= 0.0
+    {
+        forall n | n > N 
+            ensures a_i(n) >= 0.0
+        {
+            assert converges(a_i, n, 0.001, 0.001);
+        }
+    }
+
+    method exercise3_1m(a_i: pos -> real) returns (ghost negatives: set<nat>)
+        requires Limit(a_i, 0.001)
+        ensures forall x :: x in negatives ==> a_i(x) < 0.0
+        ensures exists N: nat :: positiveNat(N) && |negatives| <= N
+    {
+        var epsilon: real := 0.001;
+        assert positiveReal(epsilon);
+        ghost var N: nat :| positiveNat(N) && forall n :: n > N ==> converges(a_i, n, epsilon, 0.001);
+        ghost var i: nat := 1;
+        negatives := {};
+        while i < N
+            invariant 0 <= i <= N
+            invariant forall x :: x in negatives ==> a_i(x) < 0.0
+            invariant |negatives| <= i
+        {
+            if a_i(i) < 0.0 {
+                negatives := {i} + negatives;
+            }
+            i := i + 1;
+        }
+        assert i <= N;
+        assert |negatives| <= N;
+    }
+
+    lemma multiplyByXoverX(a: real, b: real, x: real)
+        requires x != 0.0 && b != 0.0
+        ensures a/b == prod(a,x)/prod(b,x)
+    {
+
+    }
+
+    lemma subtractLikeBase(denominator: real, x: real, y: real)
+        requires denominator != 0.0
+        ensures x/denominator-y/denominator == (x-y)/denominator
+    {
+
+    }
+
+lemma helper(x: real, y: real, z: real)
+    requires x >0.0 && y > 0.0 && z> 0.0
+    requires x * y > z * y
+    ensures x > z
+{
+
+}
+lemma biggerDenominator(bigger: nat, smaller: nat)
+    requires 0 < smaller < bigger
+    ensures (1.0 / smaller as real) > (1.0 / bigger as real)
+{
+    var delta: pos := bigger - smaller;
+    helper((1.0 / smaller as real), ((smaller+delta) as real), (1.0 / (smaller + delta) as real));
+}
+
+lemma biggerDenominatorReal(bigger: real, smaller: real)
+    requires 0.0 < smaller < bigger
+    ensures (1.0 / smaller) > (1.0 / bigger)
+{
+
+    var delta := bigger - smaller;
+    helper((1.0 / smaller as real), ((smaller+delta) as real), (1.0 / (smaller + delta) as real));
+}
+
+    function TwoNminusTwoOverFiveNPlusOne(n: pos): real {
+        (2.0*(n as real)-2.0)/(5.0*(n as real)+1.0)
+    }
+
+    lemma TwoNminusTwoOverFiveNPlusOneN(n: pos, N: pos, epsilon: real)
+        requires epsilon > 0.0
+        requires n > N
+        requires N == ((12.0/epsilon-5.0)/25.0).Floor+1
+        ensures 12.0/(25.0*(n as real)+5.0) < 12.0/(25.0*(N as real)+5.0)
+    {}
+
+    lemma {:verify } exercise3_4b() 
+        ensures Limit(TwoNminusTwoOverFiveNPlusOne, 2.0/5.0)
+    {
+
+        forall epsilon: real | positiveReal(epsilon)
+            ensures exists N: nat :: positiveNat(N) && forall n: pos :: n > N ==> converges(TwoNminusTwoOverFiveNPlusOne, n, epsilon, 2.0/5.0)
+        {
+
+    /*
+            12.0/(25.0*(n as real)+5.0) < 12.0/(25.0*(N as real)+5.0) = epsilon;
+            12.0/(25.0*(N as real)+5.0) = epsilon;
+            12.0/epsilon-5.0 = 25.0*(N as real)
+            (12.0/epsilon-5.0)/25.0 = (N as real)
+    */
+            if epsilon >= 1.0 {
+                assert positiveNat(1);
+                forall n: nat | n >1 
+                    ensures  12.0/(25.0*(n as real)+5.0) < epsilon
+                {
+    calc {
+                        abs(TwoNminusTwoOverFiveNPlusOne(n)-(2.0/5.0)) ;
+                        abs((2.0*(n as real)-2.0)/(5.0*(n as real)+1.0)-(2.0/5.0)) ;
+                        // {multiplyByXoverX(2.0, 5.0, (5.0*(n as real)+1.0));}
+                        abs((2.0*(n as real)-2.0)/(5.0*(n as real)+1.0)-prod(2.0,(5.0*(n as real)+1.0))/prod(5.0,(5.0*(n as real)+1.0))) ;
+                        abs((2.0*(n as real)-2.0)/(5.0*(n as real)+1.0)-(2.0*(5.0*(n as real)+1.0))/(5.0*(5.0*(n as real)+1.0))) ;
+                        {multiplyByXoverX(2.0*(n as real)-2.0, 5.0*(n as real)+1.0, 5.0);}
+                        abs((5.0*(2.0*(n as real)-2.0))/(5.0*(5.0*(n as real)+1.0))-(2.0*(5.0*(n as real)+1.0))/(5.0*(5.0*(n as real)+1.0))) ;
+                        abs((10.0*(n as real)-10.0)/(5.0*(5.0*(n as real)+1.0))-((10.0*(n as real)+2.0))/(5.0*(5.0*(n as real)+1.0))) ;
+                        abs((10.0*(n as real)-10.0)/(25.0*(n as real)+5.0)-(10.0*(n as real)+2.0)/(25.0*(n as real)+5.0)) ;
+                        {subtractLikeBase(25.0*(n as real)+5.0, 10.0*(n as real)-10.0, 10.0*(n as real)+2.0);}
+                        abs((10.0*(n as real)-10.0-(10.0*(n as real)+2.0))/(25.0*(n as real)+5.0)) ;
+                        abs((10.0*(n as real)-10.0-10.0*(n as real)-2.0)/(25.0*(n as real)+5.0)) ;
+                        abs((10.0*(n as real)-10.0*(n as real)-12.0)/(25.0*(n as real)+5.0)) ;
+                        abs(-12.0/(25.0*(n as real)+5.0)) ;
+                        {assert forall n : pos :: -12.0/(25.0*(n as real)+5.0) < 0.0;}
+                        -(-12.0/(25.0*(n as real)+5.0)) ;
+                        {assert forall x: real :: --x == x; assert -(-12.0/(25.0*(n as real)+5.0)) == 12.0/(25.0*(n as real)+5.0);}
+                        12.0/(25.0*(n as real)+5.0) ;
+                    }
+                    assert converges(TwoNminusTwoOverFiveNPlusOne, n, epsilon, 2.0/5.0);
+                }
+            }else{
+                var N: nat := ((12.0/epsilon-5.0)/25.0).Floor+1;
+                assert positiveNat(N);
+
+                forall n: pos | n > N
+                    ensures converges(TwoNminusTwoOverFiveNPlusOne, n, epsilon, 2.0/5.0)
+                {
+                    calc {
+                        abs(TwoNminusTwoOverFiveNPlusOne(n)-(2.0/5.0)) ;
+                        abs((2.0*(n as real)-2.0)/(5.0*(n as real)+1.0)-(2.0/5.0)) ;
+                        // {multiplyByXoverX(2.0, 5.0, (5.0*(n as real)+1.0));}
+                        abs((2.0*(n as real)-2.0)/(5.0*(n as real)+1.0)-prod(2.0,(5.0*(n as real)+1.0))/prod(5.0,(5.0*(n as real)+1.0))) ;
+                        abs((2.0*(n as real)-2.0)/(5.0*(n as real)+1.0)-(2.0*(5.0*(n as real)+1.0))/(5.0*(5.0*(n as real)+1.0))) ;
+                        {multiplyByXoverX(2.0*(n as real)-2.0, 5.0*(n as real)+1.0, 5.0);}
+                        abs((5.0*(2.0*(n as real)-2.0))/(5.0*(5.0*(n as real)+1.0))-(2.0*(5.0*(n as real)+1.0))/(5.0*(5.0*(n as real)+1.0))) ;
+                        abs((10.0*(n as real)-10.0)/(5.0*(5.0*(n as real)+1.0))-((10.0*(n as real)+2.0))/(5.0*(5.0*(n as real)+1.0))) ;
+                        abs((10.0*(n as real)-10.0)/(25.0*(n as real)+5.0)-(10.0*(n as real)+2.0)/(25.0*(n as real)+5.0)) ;
+                        {subtractLikeBase(25.0*(n as real)+5.0, 10.0*(n as real)-10.0, 10.0*(n as real)+2.0);}
+                        abs((10.0*(n as real)-10.0-(10.0*(n as real)+2.0))/(25.0*(n as real)+5.0)) ;
+                        abs((10.0*(n as real)-10.0-10.0*(n as real)-2.0)/(25.0*(n as real)+5.0)) ;
+                        abs((10.0*(n as real)-10.0*(n as real)-12.0)/(25.0*(n as real)+5.0)) ;
+                        abs(-12.0/(25.0*(n as real)+5.0)) ;
+                        {assert forall n : pos :: -12.0/(25.0*(n as real)+5.0) < 0.0;}
+                        -(-12.0/(25.0*(n as real)+5.0)) ;
+                        12.0/(25.0*(n as real)+5.0) ;
+                    }
+
+                    TwoNminusTwoOverFiveNPlusOneN(n, N, epsilon);
+                    assert 12.0/(25.0*(N as real)+5.0) < epsilon by {
+                        var niceN := ((12.0/epsilon-5.0)/25.0);
+                        var result := 12.0/(25.0*(N as real)+5.0);
+                        assert (((12.0/epsilon-5.0)/25.0).Floor+1 ) as real > niceN;
+                        assert N == (((12.0/epsilon-5.0)/25.0).Floor+1 );
+                        calc {
+                            12.0/(25.0*(((12.0/epsilon-5.0)/25.0))+5.0);
+                            12.0/(25.0*((12.0/epsilon-5.0)/25.0)+5.0);
+                            12.0/(12.0/epsilon-5.0+5.0);
+                            12.0/(12.0/epsilon);
+                            epsilon;
+
+                        }
+                        
+                        assert  (25.0*(N as real)+5.0) > (25.0*niceN+5.0);
+                        biggerDenominatorReal((25.0*(N as real)+5.0), 25.0*niceN+5.0);
+                        assert 1.0/(25.0*(N as real)+5.0) < 1.0/(25.0*(niceN)+5.0);
+                        assert (1.0/(25.0*(N as real)+5.0) )*12.0 == result;
+                        assert (1.0/(25.0*(N as real)+5.0) )*12.0 < 1.0/(25.0*(niceN)+5.0)* 12.0;
+                        assert 12.0/(25.0*(((12.0/epsilon-5.0)/25.0))+5.0) == 1.0/(25.0*(niceN)+5.0)* 12.0;
+                        assert result < 1.0/(25.0*(niceN)+5.0)* 12.0;
+                    }
+                    assert converges(TwoNminusTwoOverFiveNPlusOne, n, epsilon, 2.0/5.0);
+                }
+            }
+        }
+    }
+
+    lemma exercise3_8(a_i: pos -> real, b_i: pos -> real, a: real, b: real)
+        requires Limit(a_i, a)
+        requires Limit(b_i, b)
+        ensures Limit(addSequence(a_i, b_i), a+b)
+    {
+
+        forall epsilon: real | positiveReal(epsilon)
+            ensures exists N: nat :: positiveNat(N) && forall n: pos :: n > N ==> converges(addSequence(a_i, b_i), n, epsilon, a+b)
+        {
+            var epsilonOver2 := epsilon / 2.0;
+            assert positiveReal(epsilonOver2);
+            var N: nat :|  positiveNat(N) && forall n: pos :: n > N ==> converges(a_i, n, epsilonOver2, a);
+            var M: nat :|  positiveNat(M) && forall n: pos :: n > M ==> converges(b_i, n, epsilonOver2, b);
+            var Q := maxNat(N,M);
+            assert positiveNat(Q);
+            assert forall n: pos :: n > Q ==> converges(a_i, n, epsilonOver2, a);
+            assert forall n: pos :: n > Q ==> converges(b_i, n, epsilonOver2, b);
+            forall n: pos | n > Q 
+                ensures converges(addSequence(a_i, b_i), n, epsilon, a+b)
+            {
+                calc {
+                    abs(addSequence(a_i, b_i)(n)-(a+b));
+                    abs(a_i(n) + b_i(n)-(a+b));
+                    abs(a_i(n) + b_i(n)-a-b);
+                    abs(a_i(n) -a + b_i(n)-b);
+                }
+                assert converges(a_i, n, epsilonOver2, a);
+                assert converges(b_i, n, epsilonOver2, b);
+                assert abs(a_i(n) -a) < epsilonOver2;
+                assert abs(b_i(n)-b) < epsilonOver2;
+                assert abs(a_i(n) -a + b_i(n)-b) <= abs(a_i(n) -a) + abs(b_i(n)-b);
+            }
+        }
+    }
+
+    lemma exercise3_8b(a_i: pos -> real, a: real, c: real)
+        requires Limit(a_i, a)
+        ensures Limit(mulSequence(a_i, c), prod(c, a))
+    {
+        forall epsilon: real | positiveReal(epsilon)
+            ensures exists N: nat :: positiveNat(N) && forall n: pos :: n > N ==> converges(mulSequence(a_i, c), n, epsilon, prod(c, a))
+        {
+            if c > 0.0 {
+                var epsilonOverC := epsilon/c;
+                assert positiveReal(epsilonOverC);
+                var N: nat :|  positiveNat(N) && forall n: pos :: n > N ==> converges(a_i, n, epsilon/c, a);
+                forall n: pos | n > N 
+                    ensures converges(mulSequence(a_i, c), n, epsilon, prod(c, a))
+                {
+                    assert converges(a_i, n, epsilonOverC, a);
+                    // calc {
+                    //     abs(mulSequence(a_i, c)(n)-prod(c,a));
+                    //     abs(prod(c,a_i(n))-prod(c,a));
+                    //     abs(c*a_i(n)-c*a);
+                    //     abs(c*(a_i(n)-a));
+                    // }
+                    var dist := abs(a_i(n)-a);
+                    assert 0.0 <= dist < epsilonOverC;
+                    inequalitProduct(dist, epsilonOverC, c);
+                    assert c*0.0 <= c * dist < c * epsilonOverC;
+                    assert c * epsilon/c == epsilon;
+                    assert epsilonOverC == epsilon/c;
+                    // assert c * epsilonOverC == epsilon;
+                    // assert c*0.0 <= c * dist < epsilon;
+                    // assert 0.0 < c*epsilon;
+                    // assert c * abs(a_i(n)-a) < c*epsilon;
+                    var diff := a_i(n)-a;
+                    // absThings(diff,c);
+                    // assert c *dist == abs(c*diff);
+                    // assert c * abs(diff) == abs(c*diff); 
+                    // assert abs(c*diff) == abs(c*(a_i(n)-a));
+                    // assert abs(c*(a_i(n)-a)) < epsilon; 
+                    // assert abs(mulSequence(a_i, c)(n)-prod(c,a)) == abs(c*(a_i(n)-a));
+                    assert abs(mulSequence(a_i, c)(n)-prod(c,a)) < epsilon;
+                    assert converges(mulSequence(a_i, c), n, epsilon, prod(c, a));
+                }
+            }else if c == 0.0 {
+                var N: nat :|  positiveNat(N) && forall n: pos :: n > N ==> converges(a_i, n, epsilon, a);
+                forall n: pos | n > N 
+                    ensures converges(mulSequence(a_i, c), n, epsilon, prod(c, a))
+                {
+                }
+            }else {
+                var epsilonOverC := -epsilon/c;
+                assert positiveReal(epsilonOverC);
+                var N: nat :|  positiveNat(N) && forall n: pos :: n > N ==> converges(a_i, n, epsilonOverC, a);
+                forall n: pos | n > N 
+                    ensures converges(mulSequence(a_i, c), n, epsilon, prod(c, a))
+                {
+
+                    assert converges(a_i, n, epsilonOverC, a);
+                    // calc {
+                    //     abs(mulSequence(a_i, c)(n)-prod(c,a));
+                    //     abs(prod(c,a_i(n))-prod(c,a));
+                    //     abs(c*a_i(n)-c*a);
+                    //     abs(c*(a_i(n)-a));
+                    // }
+                    var dist := abs(a_i(n)-a);
+                    assert 0.0 <= dist < epsilonOverC;
+                    // inequalitProduct(dist, epsilonOverC, c);
+                    assert c*0.0 <= -c * dist < -c * epsilonOverC;
+                    // assert c * epsilon/c == epsilon;
+                    // assert epsilonOverC == -epsilon/c;
+                    assert -c * epsilonOverC == epsilon;
+                    assert -c*0.0 <= -c * dist < epsilon;
+                    // assert 0.0 < -c*epsilon;
+                    // assert c * abs(a_i(n)-a) < c*epsilon;
+                    var diff := a_i(n)-a;
+                    // absThings(diff,-c);
+                    // assert -c *dist == abs(c*diff);
+                    // assert -c * abs(diff) == abs(c*diff); 
+                    assert abs(c*diff) == abs(-c*(a_i(n)-a));
+                    // assert abs(c*(a_i(n)-a)) < epsilon; 
+                    assert abs(mulSequence(a_i, c)(n)-prod(c,a)) == abs(c*(a_i(n)-a));
+                    // assert abs(mulSequence(a_i, c)(n)-prod(c,a)) < epsilon;
+                    // assert converges(mulSequence(a_i, c), n, epsilon, prod(c, a));
+                }
+            }
+        }
+    }
+
+    lemma helper3(a: real, b: real)
+        requires 0.0 < a < b 
+        ensures 1.0 / a > 1.0 / b
+    {
+        var delta: real := b - a;
+    }
+
+    lemma oneOverNLessThanEpsilon(epsilon: real, N: nat) 
+        requires epsilon > 0.0
+        requires N == (1.0 / epsilon).Floor + 1
+        ensures 1.0 / N as real < epsilon
+    {
+        if epsilon > 1.0 {
+
+        }else if epsilon == 1.0 {
+            
+        }else if epsilon < 1.0 {
+            helper3(1.0/epsilon, N as real);
+            // assert 1.0 / N as real < 1.0/(1.0/epsilon);
+            assert 1.0/(1.0/epsilon) == epsilon;
+            // assert 1.0 / N as real < epsilon;
+        }
+    }
+
+    function oneOverN(n: pos): real {
+        1.0 / n as real
+    }
+
+    lemma {:verify } exercise3_9() 
+        ensures Limit(oneOverN, 0.0)
+    {
+        forall epsilon: real | positiveReal(epsilon)
+            ensures exists N: nat :: positiveNat(N) && forall n: pos :: n > N ==> converges(oneOverN, n, epsilon, 0.0)
+        {
+            var N: nat := (1.0 / epsilon).Floor + 1;
+            assert positiveNat(N);
+            forall n: pos | n > N
+                ensures converges(oneOverN, n, epsilon, 0.0)
+            {
+                biggerDenominator(n,N);
+                oneOverNLessThanEpsilon(epsilon, N);
+                assert 1.0 / N as real < epsilon;
+                assert abs(oneOverN(n)-0.0) < epsilon; //figured out that 1.0/n < 1.0/ N < epsilon
+                //figured out that f(n) < f(N) < epsilon
+            }
+        }
+    }
+
+    lemma {:verify false} exercise3_13(a_i: pos -> real, b_i: pos -> real, a: real, b: real)
+        requires Limit(a_i, a)
+        requires Limit(b_i, b)
+        ensures Limit(subSequence(a_i, b_i), a-b)
+    {
+        // exercise3_8(a_i, b_i, a, b);
+    }
+}
