Analysis/realAnalysis.dfy
@@ -1,0 +1,510 @@
+include "definitions.dfy"
+module AnalysisExercises {
+import opened Analysis
+
+
+
+lemma NaturalFraction(i: pos, k: pos)
+    requires i >= k
+    ensures 1.0/(i as real) <= 1.0/(k as real)
+{
+    if i == 1 {
+        assert k == 1;
+    }else{
+
+    }
+}
+
+lemma smallerThan1(a: real)
+    requires 0.0 < a < 1.0
+    ensures 0.0 < a*a < a < 1.0
+{
+}
+
+lemma noZeroDivisor(a: real, b: real)
+    requires a != 0.0 && b != 0.0
+    ensures a*b != 0.0
+{}
+
+lemma smallerThanR(r: real, rs: real)
+    requires 0.0 < r < 1.0
+    requires rs == r*r
+    ensures 0.0 < rs*rs < r < 1.0
+{
+    smallerThan1(r);
+    assert 0.0 < r*r < r;
+    if r*r == 0.0 {
+        noZeroDivisor(r,r);
+        assert false;
+    }
+    smallerThan1(rs);
+}
+
+lemma multLte(a: real, b: real, c: real)
+    requires c > 0.0
+    requires a < b
+    ensures a*c < b *c
+{}
+
+
+lemma uGreater(u: real, r: real)
+    requires u > 0.0 && r > 0.0
+    requires u*u > r*r
+    ensures u > r
+{
+    if u >= 1.0 {
+    }else{
+        // assert 0.0 < u < 1.0;
+        // multLte(u, 1.0, u);
+        // assert u*u < u*1.0;
+        // assert u * u < u;
+    }
+}
+
+//https://proofwiki.org/wiki/Existence_of_Square_Roots_of_Positive_Real_Number
+lemma {:vcs_split_on_every_assert} sqrtExists(r: real)
+    requires r > 0.0
+    ensures exists y :: r == y * y
+{
+    if r == 1.0 {
+        assert r == r*r;
+    }else{
+    var S := iset x | x*x < r ;
+    assert upperBound(S, r+1.0);
+    forall x | x in S 
+        ensures x < r+1.0
+    {}
+
+    forall y | y > r+1.0
+        ensures y*y !in S
+    {
+        var r' := r +1.0;
+        assert r' > 1.0;
+        assert y > 1.0;
+        assert y > r';
+    }
+    assert 0.0 in S;
+    assert forall x :: x in S ==> x < r+1.0;
+    CompletenessAxiomUpper(S,r+1.0);
+    var u :| sup(S, u);
+    if u*u > r {
+        assert u > 0.0;
+        ArchimedeanPrinciple((u*u-r)/(2.0*u));
+        assert 0.0 < (u*u-r)/(2.0*u);
+        var n: pos :| 1.0/(n as real) < (u*u-r)/(2.0*u);
+        var u' := (u-1.0/(n as real));
+        assert u' == sub(u,1.0/(n as real));
+        calc {
+            u-(u*u-r)/(2.0*u);
+            (2.0*u)*u/(2.0*u)-(u*u-r)/(2.0*u);
+            ((2.0*u)*u-(u*u-r))/(2.0*u);
+            (u*u+r)/(2.0*u);
+        }
+        assert 0.0 < 1.0/(n as real) < u;
+        assert u' > 0.0;
+        calc{
+            u'*u';
+            (u-1.0/(n as real))*(u-1.0/(n as real));
+            u*u-(2.0*u/(n as real))+1.0/((n as real)*(n as real));
+        }
+       
+        assert u'*u' > u*u-(2.0*u/(n as real));
+        assert u*u-(2.0*u/(n as real)) > r by {
+            assert (n as real) >= 1.0;
+            assert u > 0.0;
+            calc {
+                1.0/(n as real) < (u*u-r)/(2.0*u);
+                {multLte((1.0/(n as real)),((u*u-r)/(2.0*u)),2.0*u);}
+                (2.0*u)*(1.0/(n as real)) < (2.0*u)*((u*u-r)/(2.0*u));
+            }
+        }
+        assert u'*u' > r;
+        assert upperBound(S, u') by {
+            forall x | x in S
+                ensures x < u'
+            {
+                assert x*x < r < u'*u';
+                assert x*x < u'*u';
+                if x <= 0.0 {
+                }else{
+                    uGreater(u',x);
+                }
+            }
+        }
+        assert false;
+    }
+    if u*u < r {
+        assert upperBound(S, u);
+        assert u in S;
+        if u < 0.0 {
+            assert !upperBound(S, u);
+            assert false;
+        }else if u > 0.0 {
+            assert (r-u*u)/(4.0*u) > 0.0;
+            ArchimedeanPrinciple((r-u*u)/(4.0*u));
+            ArchimedeanPrinciple(2.0*u);
+            var na: pos :| 1.0 / (na as real) < ((r-u*u)/(4.0*u));
+            var nb: pos :| 1.0 / (nb as real) < (2.0*u);
+            var n := if na > nb then na else nb;
+            NaturalFraction(n, nb);
+            NaturalFraction(n, na);
+            var nf := 1.0 / (n as real);
+            assert nf > 0.0;
+            assert 1.0 / (n as real) < 2.0*u;
+            assert nf < 2.0*u;
+            assert 1.0 / (n as real) < ((r-u*u)/(4.0*u));
+            var u' := u+1.0/(n as real);
+            calc {
+                u'*u';
+                (u+1.0/(n as real))*(u+1.0/(n as real));
+                u*u+(2.0*u/(n as real))+(1.0/((n as real )*(n as real)));
+            }
+            calc {
+                nf * nf;
+                (1.0/((n as real )*(n as real)));
+            }
+            calc {
+                nf * 2.0*u;
+                (2.0*u/(n as real));
+            }
+            multLte(nf,2.0*u,nf);
+            assert nf * nf < nf *(2.0*u);
+            assert (1.0/((n as real )*(n as real))) < (2.0*u/(n as real));
+            assert u*u+(2.0*u/(n as real))+(1.0/((n as real )*(n as real))) < u*u+(2.0*u/(n as real))+(2.0*u/(n as real));
+            calc {
+                (2.0*u/(n as real))+(2.0*u/(n as real));
+                (4.0*u/(n as real));
+            }
+            assert r-u*u > 0.0;
+            assert r-u*u > (4.0*u/(n as real)) by {
+                assert 1.0 / (n as real) < ((r-u*u)/(4.0*u));
+                assert (n as real) >= 1.0;
+                calc {
+                1.0 / (n as real) < ((r-u*u)/(4.0*u));
+                (4.0*u)* (1.0 / (n as real)) < (4.0*u)*((r-u*u)/(4.0*u));
+                (4.0*u)* (1.0 / (n as real)) < (r-u*u);
+                (4.0*u / (n as real)) < (r-u*u);
+                }
+            }
+            assert u*u+(2.0*u/(n as real))+(2.0*u/(n as real)) <= u*u + (r - u*u);
+            assert u' * u' < u*u+(2.0*u/(n as real))+(2.0*u/(n as real)) <=r ;
+            assert u' * u' < r ;
+            assert u' in S;
+            assert false;
+        }else if u == 0.0 {
+            assert upperBound(S, 0.0);
+            if r > 1.0 {
+                assert 1.0 * 1.0 < r;
+                assert 1.0 in S;
+                assert false;
+            }else {
+                assert 0.0 < r < 1.0;
+                var rs := r * r;
+                smallerThanR(r,rs);
+                assert rs in S;
+                assert false;
+            }
+            assert false;
+        }
+    }
+    
+    assert u*u == r;
+    }
+}
+
+
+
+lemma stillInt(x: real) 
+    requires x.Floor as real == x
+    ensures sub(x, 1.0).Floor as real == sub(x, 1.0)
+{
+    var m: int := x.Floor;
+    assert (m-1) as real == sub(x, 1.0);
+}
+
+lemma stillIntPlus(x: real) 
+    requires x.Floor as real == x
+    ensures add(x, 1.0).Floor as real == add(x, 1.0)
+{
+    var m: int := x.Floor;
+    assert (m+1) as real == add(x, 1.0);
+}
+
+lemma floorNaturals(nats: iset<real>)
+    requires forall x :: x in nats ==> exists k: nat :: k as real == x
+    ensures forall x :: x in nats ==> x.Floor as real == x
+{
+
+}
+
+function double(n: pos): pos  {
+    2 * n
+}
+
+lemma doubleIsMonotoneInc() 
+    ensures MonotonicIncreasingPos(double)
+{}
+
+
+lemma {:verify false} TEstThing(k: nat, d_i: pos -> pos)
+    requires MonotonicIncreasingPos(d_i) 
+    // ensures exists k :: positiveNat(k) && d_i(k) > k
+{
+    assert forall n: pos :: d_i(1) <= d_i(n);
+}
+
+lemma {:verify false} sequenceConverges(a_i: pos -> real, k_i: pos -> pos, a: real)
+    ensures Limit(a_i, a) <==> forall d_i: pos -> pos :: MonotonicIncreasingPos(d_i) ==> Limit(SubSequenceOf(a_i, d_i), a)
+{
+    if Limit(a_i, a) {
+        forall d_i: pos -> pos | MonotonicIncreasingPos(d_i) 
+            ensures Limit(SubSequenceOf(a_i, d_i), a) 
+        {
+            forall epsilon: real | positiveReal(epsilon) 
+                ensures exists LN :: positiveNat(LN) && forall n :: n > LN ==> converges(SubSequenceOf(a_i, d_i), n, epsilon, a)
+            {
+                var N :| positiveNat(N) && forall n :: n > N ==> converges(a_i, n, epsilon, a);
+                var k :| positiveNat(k) && d_i(k) > N;
+            }
+        }
+    }//else if forall d_i: pos -> pos :: MonotonicIncreasingPos(d_i) && Limit(SubSequenceOf(a_i, d_i), a) {
+
+    //}
+}
+
+lemma {:verify false} MonotoneSubsequenceConverges(a_i: pos -> real, k_i: pos -> pos, a: real)
+    requires MonotonicIncreasingPos(k_i)
+    requires Monotone(a_i)
+    requires Limit(SubSequenceOf(a_i, k_i), a)
+    ensures Limit(a_i, a)
+{
+    sequenceConverges(a_i, k_i, a);
+    assert Limit(a_i, a) ==> forall d_i: pos -> pos :: MonotonicIncreasingPos(d_i) && Limit(SubSequenceOf(a_i, d_i), a);
+    assert Limit(a_i, a) <== forall d_i: pos -> pos :: MonotonicIncreasingPos(d_i) && Limit(SubSequenceOf(a_i, d_i), a);
+    if !Limit(a_i, a) {
+        if !MonotonicIncreasingPos(k_i) {
+            assert false;
+        }else if !Limit(SubSequenceOf(a_i, k_i), a) {
+            assert false;
+        }else {
+            assert MonotonicIncreasingPos(k_i) && Limit(SubSequenceOf(a_i, k_i), a) ;
+            assert !(forall d_i: pos -> pos :: MonotonicIncreasingPos(d_i) && Limit(SubSequenceOf(a_i, d_i), a));
+            assert false;
+        }
+    }
+}
+
+
+
+lemma smallerX(a: real, b : real)
+    requires a > 0.0
+    requires 0.0 <= b < 1.0
+    ensures b*a < a 
+{}
+
+lemma exercise3_18a(a_i: pos -> real, b_i: pos -> real, a_range: iset<real>, al: real, au: real)
+    requires Limit(b_i, 0.0)
+    requires a_range == iset n: pos | positiveNat(n) :: a_i(n)
+    requires al <= au
+    requires bounded(a_range, al, au) && boundedSeq(a_i, al, au)
+    ensures Limit(prodSequence(a_i, b_i), 0.0)
+{
+    assert al <= au;
+    forall epsilon: real | positiveReal(epsilon)
+        ensures exists N: nat :: positiveNat(N) && forall n: pos :: n > N ==> converges(prodSequence(a_i, b_i), n, epsilon, 0.0)
+    {
+        var max := maxReal(abs(al), abs(au))+1.0;
+        var epsilonOverMax := div(epsilon , max);
+        assert positiveReal(epsilonOverMax);
+        var N: nat :|  positiveNat(N) && forall n: pos :: n > N ==> converges(b_i, n, epsilonOverMax, 0.0);
+        forall n: pos | n > N 
+            ensures converges(prodSequence(a_i, b_i), n, epsilon,  0.0)
+        {
+            assert converges(b_i, n, epsilonOverMax, 0.0);
+            assert abs(b_i(n)-0.0) < epsilonOverMax;
+            assert abs(b_i(n)) < epsilonOverMax;
+            calc {
+            abs(prodSequence(a_i, b_i)(n)-0.0); 
+            abs(prodSequence(a_i, b_i)(n)); 
+            abs(prod(a_i(n), b_i(n))); 
+            }
+            absProd(a_i(n), b_i(n));
+            // assert prod(abs(a_i(n)) , abs(b_i(n))) == abs(prod(a_i(n), b_i(n)));
+            // assert abs(b_i(n)) < epsilonOverMax;
+            assert prod(abs(a_i(n)) , epsilonOverMax) < epsilon by {
+                assert al <= a_i(n) <= au;
+                var an := abs(a_i(n));
+                assert an >= 0.0;
+                var bx:=div(an,max); 
+                assert bx >= 0.0;
+                calc {
+                    prod(abs(a_i(n)),  div(epsilon , max));
+                    prod(an,  div(epsilon , max));
+                    {divCommute(an, epsilon, max);}
+                    prod(div(an , max) , epsilon);
+                    prod(bx , epsilon);
+                    (bx) * epsilon;
+                }
+                if abs(al) >= abs(au) {
+                    // assert abs(a_i(n)) <= abs(al) < max;
+                    divSmaller(abs(a_i(n)), max);
+                    assert abs(a_i(n))/max < 1.0;
+                    smallerX(epsilon, bx);
+                    // assert (bx) * epsilon < epsilon;
+                    // assert (abs(a_i(n)) / max) * epsilon < epsilon;
+                    // assert bx == abs(a_i(n)) / max;
+                    // assert (bx) * epsilon == prod(abs(a_i(n)) , div(epsilon , max));
+                    assert prod(abs(a_i(n)) , div(epsilon , max)) < epsilon;
+                }else{
+                    assert abs(a_i(n)) <= abs(au) < max;
+                    divSmaller(abs(a_i(n)), max);
+                    assert abs(a_i(n))/max < 1.0;
+                    // assert 0.0 <= bx < 1.0;
+                    smallerX(epsilon, bx);
+                    // assert (bx) * epsilon < epsilon;
+                    // assert (bx) * epsilon == prod(abs(a_i(n)) , div(epsilon , max));
+                    assert prod(abs(a_i(n)) , div(epsilon , max)) < epsilon;
+                }
+            }
+            // assert abs(prodSequence(a_i, b_i)(n)-0.0) ==abs(prod(a_i(n), b_i(n)));  
+            if abs(a_i(n)) == 0.0 {
+                // assert prod(abs(a_i(n)),abs(b_i(n)))  < epsilon;
+                // assert abs(prod(a_i(n), b_i(n))) < epsilon; 
+                // assert abs(prodSequence(a_i, b_i)(n)-0.0) < epsilon;
+                assert converges(prodSequence(a_i, b_i), n, epsilon, 0.0);
+            }else if abs(a_i(n)) > 0.0 {
+                // assert abs(a_i(n)) > 0.0;
+                prodLessThan(abs(a_i(n)), abs(b_i(n)), epsilonOverMax);
+                assert prod(abs(a_i(n)),abs(b_i(n))) < prod(abs(a_i(n)),epsilonOverMax) < epsilon;
+                // assert abs(prod(a_i(n), b_i(n))) < epsilon; 
+                // assert abs(prodSequence(a_i, b_i)(n)-0.0) < epsilon;
+                assert converges(prodSequence(a_i, b_i), n, epsilon, 0.0);
+            }
+        }
+
+    }
+}
+
+ghost function sqrt(x: real) : real 
+    ensures sqrt(x)*sqrt(x) == x
+
+function newtonSqrt(n: real, i: pos): real 
+    requires n > 0.0
+    requires n != 0.0
+    ensures newtonSqrt(n,i) != 0.0
+    ensures newtonSqrt(n,i) > 0.0
+    ensures n == 1.0 ==> newtonSqrt(n,i) == 1.0
+{
+    if i == 1 then 
+        assert n != 0.0;
+        n
+    else
+        var prev := newtonSqrt(n, i-1);
+        assert prev != 0.0;
+        assert (prev+(n / prev)) != 0.0;
+        (prev+(n / prev))/2.0
+}
+
+// lemma newtonSqrtGreaterThan1(n: real, i: pos)
+//     requires n > 1.0
+//     ensures newtonSqrt(n,i) > 1.0
+// {
+//     if i == 1 {
+
+//     }else{
+//         newtonSqrtGreaterThan1(n, i-1);
+
+//     }
+// }
+
+function sqrtSeq(n: real): pos -> real
+    requires n > 0.0
+{
+    (i: pos) => newtonSqrt(n,i)
+}
+
+lemma sqrtSeqLess(a: real, i: pos)
+    requires a >= 1.0
+    ensures sqrtSeq(a)(i) >= sqrtSeq(a)(i+1)
+
+lemma sqrtSeqLessAll(a: real, n: pos, m: pos)
+    requires a >= 1.0
+    requires n < m
+    ensures sqrtSeq(a)(n) >= sqrtSeq(a)(m)
+{
+    if m == n+1 {
+        sqrtSeqLess(a, n);
+        assert sqrtSeq(a)(n) >= sqrtSeq(a)(m);
+    }else{
+        assert m-1 > n;
+        sqrtSeqLessAll(a, n,m-1);
+
+        assert sqrtSeq(a)(n) >= sqrtSeq(a)(m-1);
+        sqrtSeqLess(a, m-1);
+        assert sqrtSeq(a)(n) >= sqrtSeq(a)(m);
+    }
+}
+// {
+//     if i == 0 {
+
+//     }else{
+//         var prev := sqrtSeq(a)(i);
+//         calc {
+//             sqrtSeq(a)(i+1);
+//             (prev+(a/prev))/2.0;
+//         }
+//         assert a / prev <= 1.0;
+//         assert 2.0*prev >= (prev+(a/prev));
+//         assert prev > (prev+(a/prev))/2.0;
+//     }
+// }
+
+lemma real1(a: real)
+    requires a >= 1.0
+    ensures a/a == 1.0
+{}
+
+lemma sqrtSeqMonotonic(a: real)
+    requires a >= 1.0
+    ensures MonotonicDecreasingSequence(sqrtSeq(a))
+{
+    var sseq := sqrtSeq(a);
+    forall n,m | n < m
+        ensures sseq(n) >= sseq(m)
+    {
+        if n == 1 {
+            if m == 2 {
+                calc {
+                    sseq(n);
+                    sseq(1);
+                    a;
+                }
+                real1(a);
+                assert a/a == 1.0;
+                calc {
+                    sseq(m);
+                    sseq(2);
+                    (a+a/a)/2.0;
+                    (a+1.0)/2.0;
+                }
+                // assert a >= (a+1.0)/2.0;
+                // assert sseq(1) >= a >=  (a+1.0)/2.0 >= sseq(2) ;
+                // assert sseq(1) == sseq(n);
+                // assert sseq(2) == sseq(m);
+                assert sseq(n) >= sseq(m);
+            }else{
+                assert m > 2;
+                assert sseq(n) >= sseq(m);
+            }
+        }else{
+
+            assert sseq(n) >= sseq(m);
+        }
+    }
+}
+
+    method calcSqrt(n: real) returns (nroot: real)
+    {
+    nroot := n; 
+    }
+}
